theories/Proxy.v
@@ -1,9 +1,12 @@
+Require Import FreeSpec.Concurrent.
+Require Import FreeSpec.Contract.
+Require Import FreeSpec.Control.
+Require Import FreeSpec.Control.Classes.
+Require Import FreeSpec.Control.State.
 Require Import FreeSpec.Interface.
 Require Import FreeSpec.Interp.
 Require Import FreeSpec.Program.
 Require Import FreeSpec.Refine.
-Require Import FreeSpec.Control.Classes.
-Require Import FreeSpec.Control.State.
 Require Import FreeSpec.WEq.
 
 Set Implicit Arguments.
@@ -13,7 +16,7 @@ Section PROXY.
             (S:           Type)
             (proxy:       StatefulRefinement Ii Io S)
             (to_proxy:    forall (A:  Type), I A -> option (Ii A))
-            (from_proxy:  PureRefinement Io I).
+            (from_proxy:  forall (A:  Type), Io A -> I A).
 
   Definition proxy_aux
              {A:           Type}
@@ -25,7 +28,7 @@ Section PROXY.
     | None
       => (evalInstruction int i, s, execInstruction int i)
     | Some i
-      => runProgram int (refine (proxy i s) from_proxy)
+      => runProgram int (interface_map (proxy i s) from_proxy)
     end.
 
   CoFixpoint proxify
@@ -39,4 +42,91 @@ Section PROXY.
                          (snd (fst (proxy_aux int s i)))
                )
            ).
+
+  Section ABSTRACTSPEC.
+    Variables (W:      Type)
+              (Wi Wo:  Type)
+              (c:      Contract W I)
+              (ci:     Contract Wi Ii)
+              (co:     Contract Wo Io)
+              (fi:     W -> Wi)
+              (fo:     W -> Wo)
+              (sync:   sync_pred W W S).
+
+    Definition out_req_sync
+      : Prop :=
+      forall (A:  Type)
+             (i:  Io A)
+             (w:  W),
+        requirements co i (fo w)
+        -> requirements c (from_proxy i) w.
+
+    Definition in_req_sync
+      : Prop :=
+      forall (A:   Type)
+             (i:   I A)
+             (i':  Ii A)
+             (w:   W),
+        to_proxy i = Some i'
+        -> requirements c i w
+        -> requirements ci i' (fi w).
+
+    Definition out_prom_sync
+      : Prop :=
+      forall (A:  Type)
+             (i:  Io A)
+             (x:  A)
+             (w:  W),
+        requirements co i (fo w)
+        -> promises c (from_proxy i) x w
+        -> promises co i x (fo w).
+
+    Definition in_prom_sync
+      : Prop :=
+      forall (A:   Type)
+             (i:   I A)
+             (i':  Ii A)
+             (x:   A)
+             (w:   W),
+        to_proxy i = Some i'
+        -> requirements c i w
+        -> promises ci i' x (fi w)
+        -> promises c i x w.
+
+    Definition in_unproxy_sync
+      : Prop :=
+      forall (A:   Type)
+             (i:   I A)
+             (x:   A)
+             (w:   W),
+        to_proxy i = None
+        -> requirements c i w
+        -> promises c i x w
+        -> fi w = fi (abstract_step c i x w).
+
+    Definition out_unproxy_sync
+      : Prop :=
+      forall (A:   Type)
+             (i:   I A)
+             (x:   A)
+             (w:   W),
+        to_proxy i = None
+        -> requirements c i w
+        -> promises c i x w
+        -> fo w = fo (abstract_step c i x w).
+
+    (** Our goal is to be able to prove something like that:
+
+        Theorem proxy_compliant
+                (w:  W)
+                (s:  S)
+                (int:  Interp I)
+                (Hint:  int |= c[w])
+          : proxify int s |= c[w].
+
+      By doing that, it become possible to easily adapt a component to
+      be used as a proxy. Right now, the best way to do that is to
+     *)
+
+  End ABSTRACTSPEC.
 End PROXY.
